Alphabet_Scene_Spaces.thy
@@ -110,7 +110,7 @@ qed
 definition more_frame :: "('a::scene_space \<Longrightarrow> 'b::scene_space) \<Rightarrow> 'b frame" where
 "more_frame m\<^sub>L = \<Union>\<^sub>F ((\<lambda>x. [x ;\<^sub>S m\<^sub>L]\<^sub>F) ` set Vars)"
 
-lemma more_frame_unit [simp]: "more_frame (m\<^sub>L :: unit \<Longrightarrow> 'b::scene_space) = \<lbrace>\<rbrace>"
+lemma more_frame_unit [simp]: "more_frame (m\<^sub>L :: unit \<Longrightarrow> 'b::scene_space) = \<lbrace>\<rbrace>\<^sub>F"
   by (simp add: more_frame_def)
 
 named_theorems scene_space_defs
